laying foundations of plugin vernac support for structural equivalence

src/command.ml
@@ -28,8 +28,8 @@ let arity_is_prop (mip : Declarations.one_inductive_body) : unit mm =
     @raise invalid_arity
       if lts terms and labels cannot be obtained from [mip]. [mib] is only used in case of error. *)
 let get_lts_labels_and_terms
-      (mib : Declarations.mutual_inductive_body)
-      (mip : Declarations.one_inductive_body)
+  (mib : Declarations.mutual_inductive_body)
+  (mip : Declarations.one_inductive_body)
   : (Constr.rel_declaration * Constr.rel_declaration) mm
   =
   let open Declarations in
@@ -137,9 +137,9 @@ let check_ref_lts (gref : Names.GlobRef.t) : raw_lts mm =
     - Is [w_unify] the best way?
     - ... *)
 let m_unify
-      ?(params : Params.log = default_params)
-      (t0 : EConstr.t)
-      (t1 : EConstr.t)
+  ?(params : Params.log = default_params)
+  (t0 : EConstr.t)
+  (t1 : EConstr.t)
   : bool mm
   =
   params.kind <- Debug ();
@@ -219,7 +219,7 @@ let rec pstr_int_tree (t : int tree) : string =
       lhs_int
       (List.fold_left
          (fun (acc : string) (rhs_int_tree : int tree) ->
-            pstr_int_tree rhs_int_tree)
+           pstr_int_tree rhs_int_tree)
          ""
          rhs_int_tree_list)
 ;;
@@ -228,8 +228,8 @@ let rec pstr_int_tree (t : int tree) : string =
 (* (int tree * unif_problem) list -> int tree list option t *)
 (* *)
 let rec unify_all
-          ?(params : Params.log = default_params)
-          (i : (int tree * unif_problem) list)
+  ?(params : Params.log = default_params)
+  (i : (int tree * unif_problem) list)
   : int tree list option t
   =
   params.kind <- Debug ();
@@ -257,9 +257,9 @@ let rec unify_all
 ;;
 
 let sandboxed_unify
-      ?(params : Params.log = default_params)
-      (tgt_term : EConstr.t)
-      (u : (int tree * unif_problem) list)
+  ?(params : Params.log = default_params)
+  (tgt_term : EConstr.t)
+  (u : (int tree * unif_problem) list)
   : (EConstr.t * int tree list) option mm
   =
   params.kind <- Debug ();
@@ -282,11 +282,11 @@ let sandboxed_unify
 
 (* [act] should probably come from the unification problems? *)
 let rec retrieve_tgt_nodes
-          ?(params : Params.log = default_params)
-          (acc : (EConstr.t * EConstr.t * int tree) list)
-          (i : int)
-          (act : EConstr.t)
-          (tgt_term : EConstr.t)
+  ?(params : Params.log = default_params)
+  (acc : (EConstr.t * EConstr.t * int tree) list)
+  (i : int)
+  (act : EConstr.t)
+  (tgt_term : EConstr.t)
   :  (int tree * unif_problem) list list
   -> (EConstr.t * EConstr.t * int tree) list t
   =
@@ -310,9 +310,9 @@ let rec retrieve_tgt_nodes
 
 (* Should return a list of unification problems *)
 let rec check_updated_ctx
-          ?(params : Params.log = default_params)
-          (acc : (int tree * unif_problem) list list)
-          (rlts_ctx : rlts_list)
+  ?(params : Params.log = default_params)
+  (acc : (int tree * unif_problem) list list)
+  (rlts_ctx : rlts_list)
   :  EConstr.t list * EConstr.rel_declaration list
   -> (int tree * unif_problem) list list option t
   = function
@@ -341,7 +341,7 @@ let rec check_updated_ctx
             let ctors =
               List.map
                 (fun (_, (tL : EConstr.t), (i : int tree)) ->
-                   i, { termL = tL; termR = args.(2) })
+                  i, { termL = tL; termR = args.(2) })
                 ctors
             in
             (* We need to cross-product all possible unifications. This is in case
@@ -365,11 +365,11 @@ let rec check_updated_ctx
 
 (** Checks possible transitions for this term: *)
 and check_valid_constructor
-      ?(params : Params.log = default_params)
-      (rlts : raw_lts)
-      (rlts_ctx : rlts_list)
-      (t : EConstr.t)
-      (ma : EConstr.t option)
+  ?(params : Params.log = default_params)
+  (rlts : raw_lts)
+  (rlts_ctx : rlts_list)
+  (t : EConstr.t)
+  (ma : EConstr.t option)
   : (EConstr.t * EConstr.t * int tree) list t
   =
   params.kind <- Debug ();
@@ -439,8 +439,8 @@ module type GraphB = sig
 
   type lts_graph =
     { to_visit : EConstr.constr Queue.t
-      (* Queue for BFS *)
-      (* ; labels : L.t *)
+        (* Queue for BFS *)
+        (* ; labels : L.t *)
     ; states : S.t
     ; transitions : lts_transition H.t
     }
@@ -541,10 +541,10 @@ struct
       @param g is an [lts_graph] accumulated while exploring [rlts].
       @return an [lts_graph] constructed so long as the [bound] is not exceeded. *)
   let rec build_lts_graph
-            ?(params : Params.log = default_params)
-            (rlts_ctx : rlts_list)
-            (g : lts_graph)
-            (bound : int)
+    ?(params : Params.log = default_params)
+    (rlts_ctx : rlts_list)
+    (g : lts_graph)
+    (bound : int)
     : lts_graph mm
     =
     params.kind <- Debug ();
@@ -559,20 +559,18 @@ struct
         List.fold_left
           (fun (acc : (EConstr.t * EConstr.t * int tree) list t)
             (rlts : raw_lts) ->
-             let* ctors =
-               check_valid_constructor ~params rlts rlts_ctx t None
-             in
-             if List.is_empty ctors
-             then acc
-             else
-               return
-                 (List.fold_left
-                    (fun (acc' : (EConstr.t * EConstr.t * int tree) list)
-                      (ctor : EConstr.t * EConstr.t * int tree) ->
-                       (* TODO: figure out how to  merge *)
-                       ctor :: acc')
-                    (run acc)
-                    ctors))
+            let* ctors = check_valid_constructor ~params rlts rlts_ctx t None in
+            if List.is_empty ctors
+            then acc
+            else
+              return
+                (List.fold_left
+                   (fun (acc' : (EConstr.t * EConstr.t * int tree) list)
+                     (ctor : EConstr.t * EConstr.t * int tree) ->
+                     (* TODO: figure out how to  merge *)
+                     ctor :: acc')
+                   (run acc)
+                   ctors))
           (return [])
           rlts_ctx
       in
@@ -587,12 +585,12 @@ struct
                  (List.fold_left
                     (fun (acc : string)
                       ((act, ctor, int_tree) : EConstr.t * EConstr.t * int tree) ->
-                       Printf.sprintf
-                         "%s   (%s ::\n    %s[%s])\n"
-                         acc
-                         (pstr_int_tree int_tree)
-                         (econstr_to_string ctor)
-                         (econstr_to_string act))
+                      Printf.sprintf
+                        "%s   (%s ::\n    %s[%s])\n"
+                        acc
+                        (pstr_int_tree int_tree)
+                        (econstr_to_string ctor)
+                        (econstr_to_string act))
                     "\n"
                     constrs)
                  (List.length constrs)))
@@ -609,27 +607,27 @@ struct
       let* sigma = get_sigma in
       List.iter
         (fun ((act, tgt, int_tree) : EConstr.t * EConstr.t * int tree) ->
-           log
-             ~params
-             (Printf.sprintf "\n\nTransition to: %s." (econstr_to_string tgt));
-           new_states := S.add tgt !new_states;
-           (* TODO: detect tau transitions and then defer to [Fsm.tau] instead. *)
-           let to_add : action =
-             Fsm.Create.action
-               ~is_tau:false
-               ~annotation:[]
-               (Of (get_transition_id (), econstr_to_string act))
-           in
-           H.add
-             g.transitions
-             t
-             { action = to_add; index_tree = int_tree; destination = tgt };
-           if H.mem g.transitions tgt || EConstr.eq_constr sigma tgt t
-           then ()
-           else Queue.push tgt g.to_visit;
-           log
-             ~params
-             (Printf.sprintf "\nVisiting next: %i." (Queue.length g.to_visit)))
+          log
+            ~params
+            (Printf.sprintf "\n\nTransition to: %s." (econstr_to_string tgt));
+          new_states := S.add tgt !new_states;
+          (* TODO: detect tau transitions and then defer to [Fsm.tau] instead. *)
+          let to_add : action =
+            Fsm.Create.action
+              ~is_tau:false
+              ~annotation:[]
+              (Of (get_transition_id (), econstr_to_string act))
+          in
+          H.add
+            g.transitions
+            t
+            { action = to_add; index_tree = int_tree; destination = tgt };
+          if H.mem g.transitions tgt || EConstr.eq_constr sigma tgt t
+          then ()
+          else Queue.push tgt g.to_visit;
+          log
+            ~params
+            (Printf.sprintf "\nVisiting next: %i." (Queue.length g.to_visit)))
         constrs;
       let g = { g with states = S.union g.states !new_states } in
       build_lts_graph ~params rlts_ctx g bound
@@ -649,10 +647,10 @@ struct
       @param rlts is the raw_lts of the inductively defined coq term.
       @param t is the original Coq-term. *)
   let build_graph
-        ?(params : Params.log = default_params)
-        (rlts_ctx : rlts_list)
-        (t : Constrexpr.constr_expr_r CAst.t)
-        (bound : int)
+    ?(params : Params.log = default_params)
+    (rlts_ctx : rlts_list)
+    (t : Constrexpr.constr_expr_r CAst.t)
+    (bound : int)
     : lts_graph mm
     =
     let$ t env sigma = Constrintern.interp_constr_evars env sigma t in
@@ -688,8 +686,8 @@ struct
     (* TODO: refactor pstr_lts and others *)
 
     let constructor
-          ?(params : Params.pstr = Fmt (Params.Default.fmt ~mode:(Coq ()) ()))
-          (t : lts_transition)
+      ?(params : Params.pstr = Fmt (Params.Default.fmt ~mode:(Coq ()) ()))
+      (t : lts_transition)
       : string mm
       =
       let _params : Params.fmt = Params.handle params in
@@ -705,8 +703,8 @@ struct
     ;;
 
     let transition
-          ?(params : Params.pstr = Fmt (Params.Default.fmt ~mode:(Coq ()) ()))
-          ((from, transition) : EConstr.constr * lts_transition)
+      ?(params : Params.pstr = Fmt (Params.Default.fmt ~mode:(Coq ()) ()))
+      ((from, transition) : EConstr.constr * lts_transition)
       : string mm
       =
       let _params : Params.fmt = Params.handle params in
@@ -733,8 +731,8 @@ struct
     ;;
 
     let transitions
-          ?(params : Params.pstr = Fmt (Params.Default.fmt ~mode:(Coq ()) ()))
-          (transitions : lts_transition H.t)
+      ?(params : Params.pstr = Fmt (Params.Default.fmt ~mode:(Coq ()) ()))
+      (transitions : lts_transition H.t)
       : string mm
       =
       let _params : Params.fmt = Params.handle params in
@@ -748,11 +746,11 @@ struct
             (fun (from : EConstr.t)
               (transition' : lts_transition)
               (acc : string) ->
-               Printf.sprintf
-                 "%s%s%s\n"
-                 acc
-                 tabs'
-                 (run (transition (from, transition'))))
+              Printf.sprintf
+                "%s%s%s\n"
+                acc
+                tabs'
+                (run (transition (from, transition'))))
             transitions
             "\n"
         in
@@ -760,8 +758,8 @@ struct
     ;;
 
     let states
-          ?(params : Params.pstr = Fmt (Params.Default.fmt ~mode:(Coq ()) ()))
-          (states : N.t)
+      ?(params : Params.pstr = Fmt (Params.Default.fmt ~mode:(Coq ()) ()))
+      (states : N.t)
       : string mm
       =
       let _params : Params.fmt = Params.handle params in
@@ -773,7 +771,7 @@ struct
         let pstr : string =
           N.fold
             (fun (s : EConstr.t) (acc : string) ->
-               Printf.sprintf "%s%s%s\n" acc tabs' (run (econstr s)))
+              Printf.sprintf "%s%s%s\n" acc tabs' (run (econstr s)))
             states
             "\n"
         in
@@ -781,8 +779,8 @@ struct
     ;;
 
     let queue
-          ?(params : Params.pstr = Fmt (Params.Default.fmt ~mode:(Coq ()) ()))
-          (q : EConstr.t Queue.t)
+      ?(params : Params.pstr = Fmt (Params.Default.fmt ~mode:(Coq ()) ()))
+      (q : EConstr.t Queue.t)
       : string mm
       =
       let _params : Params.fmt = Params.handle params in
@@ -794,7 +792,7 @@ struct
         let pstr : string =
           Queue.fold
             (fun (acc : string) (to_visit : EConstr.t) ->
-               Printf.sprintf "%s%s%s\n" acc tabs' (run (econstr to_visit)))
+              Printf.sprintf "%s%s%s\n" acc tabs' (run (econstr to_visit)))
             "\n"
             q
         in
@@ -802,8 +800,8 @@ struct
     ;;
 
     let lts
-          ?(params : Params.pstr = Fmt (Params.Default.fmt ~mode:(Coq ()) ()))
-          (g : lts_graph)
+      ?(params : Params.pstr = Fmt (Params.Default.fmt ~mode:(Coq ()) ()))
+      (g : lts_graph)
       : string mm
       =
       let _params : Params.fmt = Params.handle params in
@@ -868,28 +866,28 @@ struct
     (* type coq_translation = coq_translation_record mm *)
 
     let translate_coq_terms
-          ?(params : Params.log = default_params)
-          (states : N.t)
+      ?(params : Params.log = default_params)
+      (states : N.t)
       : coq_translation mm
       =
       let tbl : coq_translation = make_coq_translation in
       S.iter
         (fun (s : EConstr.t) ->
-           match Hashtbl.find_opt tbl.from_coq s with
-           | None ->
-             (* add as new state *)
-             let str : string = econstr_to_string s in
-             Hashtbl.add tbl.from_coq s str;
-             Hashtbl.add tbl.to_coq str s
-           | Some _ -> (* ignore *) ())
+          match Hashtbl.find_opt tbl.from_coq s with
+          | None ->
+            (* add as new state *)
+            let str : string = econstr_to_string s in
+            Hashtbl.add tbl.from_coq s str;
+            Hashtbl.add tbl.to_coq str s
+          | Some _ -> (* ignore *) ())
         states;
       return tbl
     ;;
 
     let translate_coq_lts
-          ?(params : Params.log = default_params)
-          (transitions : lts_transition H.t)
-          (tbl : coq_translation)
+      ?(params : Params.log = default_params)
+      (transitions : lts_transition H.t)
+      (tbl : coq_translation)
       : Lts.raw_flat_lts mm
       =
       return
@@ -897,17 +895,17 @@ struct
            (fun (from : EConstr.t)
              (transition : (action, EConstr.constr) transition)
              (acc : Lts.raw_flat_lts) ->
-              ( Hashtbl.find tbl.from_coq from
-              , transition.action.label
-              , Hashtbl.find tbl.from_coq transition.destination )
-              :: acc)
+             ( Hashtbl.find tbl.from_coq from
+             , transition.action.label
+             , Hashtbl.find tbl.from_coq transition.destination )
+             :: acc)
            transitions
            [])
     ;;
 
     let translate_init_term
-          (init_term : Constrexpr.constr_expr_r CAst.t)
-          (tbl : coq_translation)
+      (init_term : Constrexpr.constr_expr_r CAst.t)
+      (tbl : coq_translation)
       : string mm
       =
       let$ t env sigma = Constrintern.interp_constr_evars env sigma init_term in
@@ -920,11 +918,11 @@ struct
     (* exception UnfinishedLTS of lts_graph *)
 
     let lts_graph_to_lts
-          ?(params : Params.log = default_params)
-          ?(bound : int = default_bound)
-          ?(name : string = "unknown")
-          (g : lts_graph)
-          (init_term : Constrexpr.constr_expr_r CAst.t)
+      ?(params : Params.log = default_params)
+      ?(bound : int = default_bound)
+      ?(name : string = "unknown")
+      (g : lts_graph)
+      (init_term : Constrexpr.constr_expr_r CAst.t)
       : (Lts.lts * coq_translation) mm
       =
       params.kind <- Debug ();
@@ -994,30 +992,30 @@ let make_graph_builder =
 
 (** *)
 let build_rlts_ctx
-      ?(params : Params.log = default_params)
-      (grefs : Names.GlobRef.t list)
+  ?(params : Params.log = default_params)
+  (grefs : Names.GlobRef.t list)
   : rlts_list
   =
   List.fold_left
     (fun (acc : rlts_list) (gref : Names.GlobRef.t) ->
-       let rlts : raw_lts = run (check_ref_lts gref) in
-       log
-         ~params
-         (Printf.sprintf "= = = = = = = = =\n\trlts (#%d):" (List.length acc));
-       let _ = log_raw_lts ~params rlts in
-       List.append acc [ rlts ])
+      let rlts : raw_lts = run (check_ref_lts gref) in
+      log
+        ~params
+        (Printf.sprintf "= = = = = = = = =\n\trlts (#%d):" (List.length acc));
+      let _ = log_raw_lts ~params rlts in
+      List.append acc [ rlts ])
     []
     grefs
 ;;
 
 (** *)
 let build_bounded_lts
-      ?(params : Params.log = default_params)
-      ?(bound : int = default_bound)
-      ?(name : string = "unknown")
-      (rlts_ctx : raw_lts list)
-      (tref : Constrexpr.constr_expr_r CAst.t)
-      (module G : GraphB)
+  ?(params : Params.log = default_params)
+  ?(bound : int = default_bound)
+  ?(name : string = "unknown")
+  (rlts_ctx : raw_lts list)
+  (tref : Constrexpr.constr_expr_r CAst.t)
+  (module G : GraphB)
   : Lts.lts mm
   =
   (* graph lts *)
@@ -1054,11 +1052,11 @@ let build_bounded_lts
 
 (** *)
 let build_fsm_from_bounded_lts
-      ?(params : Params.log = default_params)
-      ?(bound : int = default_bound)
-      ?(name : string = "unknown")
-      (tref : Constrexpr.constr_expr_r CAst.t)
-      (grefs : Names.GlobRef.t list)
+  ?(params : Params.log = default_params)
+  ?(bound : int = default_bound)
+  ?(name : string = "unknown")
+  (tref : Constrexpr.constr_expr_r CAst.t)
+  (grefs : Names.GlobRef.t list)
   : Fsm.fsm mm
   =
   (* disable detailed printouts *)
@@ -1080,11 +1078,12 @@ let build_fsm_from_bounded_lts
 module Vernac = struct
   module LTS = struct
     let build
-          ?(params : Params.log = default_params)
-          ?(bound : int = default_bound)
-          ?(name : string = "unknown")
-          (tref : Constrexpr.constr_expr_r CAst.t)
-          (grefs : Names.GlobRef.t list)
+      ?(params : Params.log = default_params)
+      ?(bound : int = default_bound)
+      ?(name : string = "unknown")
+      ?(equiv : Names.GlobRef.t option)
+      (tref : Constrexpr.constr_expr_r CAst.t)
+      (grefs : Names.GlobRef.t list)
       : Lts.lts mm
       =
       (* list of raw coq lts *)
@@ -1097,10 +1096,11 @@ module Vernac = struct
     ;;
 
     let show
-          ?(params : Params.log = default_params)
-          ?(bound : int = default_bound)
-          (tref : Constrexpr.constr_expr_r CAst.t)
-          (grefs : Names.GlobRef.t list)
+      ?(params : Params.log = default_params)
+      ?(bound : int = default_bound)
+      ?(equiv : Names.GlobRef.t option)
+      (tref : Constrexpr.constr_expr_r CAst.t)
+      (grefs : Names.GlobRef.t list)
       : unit mm
       =
       let* (the_lts : Lts.lts) = build ~params ~bound tref grefs in
@@ -1113,11 +1113,12 @@ module Vernac = struct
     ;;
 
     let dump
-          ?(params : Params.log = default_params)
-          ?(bound : int = default_bound)
-          ?(name : string = "dump")
-          (tref : Constrexpr.constr_expr_r CAst.t)
-          (grefs : Names.GlobRef.t list)
+      ?(params : Params.log = default_params)
+      ?(bound : int = default_bound)
+      ?(name : string = "dump")
+      ?(equiv : Names.GlobRef.t option)
+      (tref : Constrexpr.constr_expr_r CAst.t)
+      (grefs : Names.GlobRef.t list)
       : unit mm
       =
       params.options.output_enabled <- false;
@@ -1148,21 +1149,23 @@ module Vernac = struct
   module FSM = struct
     (** *)
     let build
-          ?(params : Params.log = default_params)
-          ?(bound : int = default_bound)
-          ?(name : string = "unknown")
-          (tref : Constrexpr.constr_expr_r CAst.t)
-          (grefs : Names.GlobRef.t list)
+      ?(params : Params.log = default_params)
+      ?(bound : int = default_bound)
+      ?(name : string = "unknown")
+      ?(equiv : Names.GlobRef.t option)
+      (tref : Constrexpr.constr_expr_r CAst.t)
+      (grefs : Names.GlobRef.t list)
       : Fsm.fsm mm
       =
       build_fsm_from_bounded_lts ~params ~bound ~name tref grefs
     ;;
 
     let show
-          ?(params : Params.log = default_params)
-          ?(bound : int = default_bound)
-          (tref : Constrexpr.constr_expr_r CAst.t)
-          (grefs : Names.GlobRef.t list)
+      ?(params : Params.log = default_params)
+      ?(bound : int = default_bound)
+      ?(equiv : Names.GlobRef.t option)
+      (tref : Constrexpr.constr_expr_r CAst.t)
+      (grefs : Names.GlobRef.t list)
       : unit mm
       =
       (* get translated fsm *)
@@ -1178,11 +1181,12 @@ module Vernac = struct
     ;;
 
     let dump
-          ?(params : Params.log = default_params)
-          ?(bound : int = default_bound)
-          ?(name : string = "dump")
-          (tref : Constrexpr.constr_expr_r CAst.t)
-          (grefs : Names.GlobRef.t list)
+      ?(params : Params.log = default_params)
+      ?(bound : int = default_bound)
+      ?(name : string = "dump")
+      ?(equiv : Names.GlobRef.t option)
+      (tref : Constrexpr.constr_expr_r CAst.t)
+      (grefs : Names.GlobRef.t list)
       : unit mm
       =
       (* get translated fsm *)
@@ -1202,11 +1206,11 @@ module Vernac = struct
   module Minim = struct
     (** *)
     let build
-          ?(params : Params.log = default_params)
-          ?(bound : int = default_bound)
-          ?(name : string = "unknown")
-          (tref : Constrexpr.constr_expr_r CAst.t)
-          (grefs : Names.GlobRef.t list)
+      ?(params : Params.log = default_params)
+      ?(bound : int = default_bound)
+      ?(name : string = "unknown")
+      (tref : Constrexpr.constr_expr_r CAst.t)
+      (grefs : Names.GlobRef.t list)
       : (Fsm.fsm * Fsm.fsm) mm
       =
       (* get translated fsm *)
@@ -1219,10 +1223,10 @@ module Vernac = struct
 
     (** *)
     let show
-          ?(params : Params.log = default_params)
-          ?(bound : int = default_bound)
-          (tref : Constrexpr.constr_expr_r CAst.t)
-          (grefs : Names.GlobRef.t list)
+      ?(params : Params.log = default_params)
+      ?(bound : int = default_bound)
+      (tref : Constrexpr.constr_expr_r CAst.t)
+      (grefs : Names.GlobRef.t list)
       : unit mm
       =
       (* get translated fsm *)
@@ -1241,11 +1245,11 @@ module Vernac = struct
     ;;
 
     let dump
-          ?(params : Params.log = default_params)
-          ?(bound : int = default_bound)
-          ?(name : string = "dump")
-          (tref : Constrexpr.constr_expr_r CAst.t)
-          (grefs : Names.GlobRef.t list)
+      ?(params : Params.log = default_params)
+      ?(bound : int = default_bound)
+      ?(name : string = "dump")
+      (tref : Constrexpr.constr_expr_r CAst.t)
+      (grefs : Names.GlobRef.t list)
       : unit mm
       =
       (* get translated fsm *)
@@ -1276,12 +1280,12 @@ module Vernac = struct
   module Merged = struct
     (** *)
     let build
-          ?(params : Params.log = default_params)
-          ?(bound : int = default_bound)
-          ?(name : string = "unknown")
-          (trefA : Constrexpr.constr_expr_r CAst.t)
-          (trefB : Constrexpr.constr_expr_r CAst.t)
-          (grefs : Names.GlobRef.t list)
+      ?(params : Params.log = default_params)
+      ?(bound : int = default_bound)
+      ?(name : string = "unknown")
+      (trefA : Constrexpr.constr_expr_r CAst.t)
+      (trefB : Constrexpr.constr_expr_r CAst.t)
+      (grefs : Names.GlobRef.t list)
       : (Fsm.fsm * Fsm.fsm * Fsm.fsm) mm
       =
       (* get translated fsm *)
@@ -1300,11 +1304,11 @@ module Vernac = struct
 
     (** *)
     let show
-          ?(params : Params.log = default_params)
-          ?(bound : int = default_bound)
-          (trefA : Constrexpr.constr_expr_r CAst.t)
-          (trefB : Constrexpr.constr_expr_r CAst.t)
-          (grefs : Names.GlobRef.t list)
+      ?(params : Params.log = default_params)
+      ?(bound : int = default_bound)
+      (trefA : Constrexpr.constr_expr_r CAst.t)
+      (trefB : Constrexpr.constr_expr_r CAst.t)
+      (grefs : Names.GlobRef.t list)
       : unit mm
       =
       (* get merged fsm *)
@@ -1324,12 +1328,12 @@ module Vernac = struct
     ;;
 
     let dump
-          ?(params : Params.log = default_params)
-          ?(bound : int = default_bound)
-          ?(name : string = "dump")
-          (trefA : Constrexpr.constr_expr_r CAst.t)
-          (trefB : Constrexpr.constr_expr_r CAst.t)
-          (grefs : Names.GlobRef.t list)
+      ?(params : Params.log = default_params)
+      ?(bound : int = default_bound)
+      ?(name : string = "dump")
+      (trefA : Constrexpr.constr_expr_r CAst.t)
+      (trefB : Constrexpr.constr_expr_r CAst.t)
+      (grefs : Names.GlobRef.t list)
       : unit mm
       =
       (* get merged fsm *)
@@ -1373,12 +1377,12 @@ module Vernac = struct
 
     (** *)
     let build
-          ?(params : Params.log = default_params)
-          ?(bound : int = default_bound)
-          ?(name : string = "unknown")
-          (trefA : Constrexpr.constr_expr_r CAst.t)
-          (trefB : Constrexpr.constr_expr_r CAst.t)
-          (grefs : Names.GlobRef.t list)
+      ?(params : Params.log = default_params)
+      ?(bound : int = default_bound)
+      ?(name : string = "unknown")
+      (trefA : Constrexpr.constr_expr_r CAst.t)
+      (trefB : Constrexpr.constr_expr_r CAst.t)
+      (grefs : Names.GlobRef.t list)
       : (Fsm.fsm * Fsm.fsm * Bisimilarity.result) mm
       =
       (* get translated fsm *)
@@ -1396,11 +1400,11 @@ module Vernac = struct
 
     (** *)
     let show
-          ?(params : Params.log = default_params)
-          ?(bound : int = default_bound)
-          (trefA : Constrexpr.constr_expr_r CAst.t)
-          (trefB : Constrexpr.constr_expr_r CAst.t)
-          (grefs : Names.GlobRef.t list)
+      ?(params : Params.log = default_params)
+      ?(bound : int = default_bound)
+      (trefA : Constrexpr.constr_expr_r CAst.t)
+      (trefB : Constrexpr.constr_expr_r CAst.t)
+      (grefs : Names.GlobRef.t list)
       : unit mm
       =
       let* fsm_A, fsm_B, result = build ~params ~bound trefA trefB grefs in
@@ -1421,12 +1425,12 @@ module Vernac = struct
     ;;
 
     let dump
-          ?(params : Params.log = default_params)
-          ?(bound : int = default_bound)
-          ?(name : string = "dump")
-          (trefA : Constrexpr.constr_expr_r CAst.t)
-          (trefB : Constrexpr.constr_expr_r CAst.t)
-          (grefs : Names.GlobRef.t list)
+      ?(params : Params.log = default_params)
+      ?(bound : int = default_bound)
+      ?(name : string = "dump")
+      (trefA : Constrexpr.constr_expr_r CAst.t)
+      (trefB : Constrexpr.constr_expr_r CAst.t)
+      (grefs : Names.GlobRef.t list)
       : unit mm
       =
       let* fsm_A, fsm_B, result =
