src/command.mli
@@ -4,6 +4,7 @@ module Vernac : sig
       :  ?params:Utils.Logging.params
       -> ?bound:int
       -> ?name:string
+      -> ?equiv:Names.GlobRef.t
       -> Constrexpr.constr_expr_r CAst.t
       -> Names.GlobRef.t list
       -> Lts.lts Mebi_monad.t
@@ -11,6 +12,7 @@ module Vernac : sig
     val show
       :  ?params:Utils.Logging.params
       -> ?bound:int
+      -> ?equiv:Names.GlobRef.t
       -> Constrexpr.constr_expr_r CAst.t
       -> Names.GlobRef.t list
       -> unit Mebi_monad.t
@@ -19,6 +21,7 @@ module Vernac : sig
       :  ?params:Utils.Logging.params
       -> ?bound:int
       -> ?name:string
+      -> ?equiv:Names.GlobRef.t
       -> Constrexpr.constr_expr_r CAst.t
       -> Names.GlobRef.t list
       -> unit Mebi_monad.t
@@ -29,6 +32,7 @@ module Vernac : sig
       :  ?params:Utils.Logging.params
       -> ?bound:int
       -> ?name:string
+      -> ?equiv:Names.GlobRef.t
       -> Constrexpr.constr_expr_r CAst.t
       -> Names.GlobRef.t list
       -> Fsm.fsm Mebi_monad.t
@@ -36,6 +40,7 @@ module Vernac : sig
     val show
       :  ?params:Utils.Logging.params
       -> ?bound:int
+      -> ?equiv:Names.GlobRef.t
       -> Constrexpr.constr_expr_r CAst.t
       -> Names.GlobRef.t list
       -> unit Mebi_monad.t
@@ -44,6 +49,7 @@ module Vernac : sig
       :  ?params:Utils.Logging.params
       -> ?bound:int
       -> ?name:string
+      -> ?equiv:Names.GlobRef.t
       -> Constrexpr.constr_expr_r CAst.t
       -> Names.GlobRef.t list
       -> unit Mebi_monad.t
